Changed uniform.

vsSahlq_ITP/coq_code/pos.v
@@ -1,9 +1,9 @@
 Require Import p_is_pos p_is_neg.
 
-Definition uniform_pos (ϕ : Modal) : Prop :=
+Definition pos (ϕ : Modal) : Prop :=
 forall p, pv_in_modal ϕ p -> p_is_pos ϕ p.
 
-Definition uniform_neg (ϕ : Modal) : Prop :=
+Definition neg (ϕ : Modal) : Prop :=
 forall p, pv_in_modal ϕ p -> p_is_neg ϕ p.
 
 Definition uniform (ϕ : Modal) : Prop :=
